<?xml version="1.0" encoding="utf-8"?>
<rdf:RDF
   xmlns:dc="http://purl.org/dc/elements/1.1/"
   xmlns:rdf="http://www.w3.org/1999/02/22-rdf-syntax-ns#"
   xmlns:skos="http://www.w3.org/2004/02/skos/core#"
>
  <rdf:Description rdf:about="https://vocab.inidep.edu.ar/organizaciones/UBA">
    <rdf:type rdf:resource="http://www.w3.org/2004/02/skos/core#Concept"/>
    <skos:inScheme rdf:resource="https://vocab.inidep.edu.ar/organizaciones/"/>
    <skos:prefLabel xml:lang="es">Universidad de Buenos Aires</skos:prefLabel>
    <skos:prefLabel xml:lang="en">University of Buenos Aires</skos:prefLabel>
    <skos:definition xml:lang="es">Principal universidad pública de Argentina, con una amplia gama de programas de investigación, incluyendo ciencias del mar.</skos:definition>
    <skos:definition xml:lang="en">The main public university in Argentina, with a wide range of research programs, including marine sciences.</skos:definition>
    <skos:altLabel xml:lang="en">UBA</skos:altLabel>
    <dc:source>https://www.uba.ar/</dc:source>
  </rdf:Description>
  <rdf:Description rdf:about="https://vocab.inidep.edu.ar/organizaciones/CIMAS">
    <rdf:type rdf:resource="http://www.w3.org/2004/02/skos/core#Concept"/>
    <skos:inScheme rdf:resource="https://vocab.inidep.edu.ar/organizaciones/"/>
    <skos:prefLabel xml:lang="es">Centro de Investigación Aplicada y Transferencia Tecnológica en Recursos Marinos Alte. Storni</skos:prefLabel>
    <skos:prefLabel xml:lang="en">Alte. Storni Center for Applied Research and Technology Transfer in Marine Resources</skos:prefLabel>
    <skos:definition xml:lang="es">Instituto de investigación en San Antonio Oeste, Argentina, enfocado en la acuicultura y los recursos marinos patagónicos.</skos:definition>
    <skos:definition xml:lang="en">Research institute in San Antonio Oeste, Argentina, focused on aquaculture and Patagonian marine resources.</skos:definition>
    <skos:altLabel xml:lang="en">CIMAS</skos:altLabel>
    <dc:source>https://cimas.org.ar/</dc:source>
  </rdf:Description>
  <rdf:Description rdf:about="https://vocab.inidep.edu.ar/organizaciones/IAA">
    <rdf:type rdf:resource="http://www.w3.org/2004/02/skos/core#Concept"/>
    <skos:inScheme rdf:resource="https://vocab.inidep.edu.ar/organizaciones/"/>
    <skos:prefLabel xml:lang="es">Instituto Antártico Argentino</skos:prefLabel>
    <skos:prefLabel xml:lang="en">Argentine Antarctic Institute</skos:prefLabel>
    <skos:definition xml:lang="es">Organismo gubernamental de Argentina que centraliza la planificación y ejecución de la investigación científica en la Antártida.</skos:definition>
    <skos:definition xml:lang="en">Governmental body of Argentina that centralizes the planning and execution of scientific research in Antarctica.</skos:definition>
    <skos:altLabel xml:lang="en">IAA</skos:altLabel>
    <dc:source>https://www.argentina.gob.ar/ciencia/iaa</dc:source>
  </rdf:Description>
  <rdf:Description rdf:about="https://vocab.inidep.edu.ar/organizaciones/CONICET">
    <rdf:type rdf:resource="http://www.w3.org/2004/02/skos/core#Concept"/>
    <skos:inScheme rdf:resource="https://vocab.inidep.edu.ar/organizaciones/"/>
    <skos:prefLabel xml:lang="es">Consejo Nacional de Investigaciones Científicas y Técnicas</skos:prefLabel>
    <skos:prefLabel xml:lang="en">National Scientific and Technical Research Council</skos:prefLabel>
    <skos:definition xml:lang="es">Principal organismo de Argentina dedicado a la promoción de la ciencia y la tecnología.</skos:definition>
    <skos:definition xml:lang="en">The main agency in Argentina dedicated to the promotion of science and technology.</skos:definition>
    <skos:altLabel xml:lang="en">CONICET</skos:altLabel>
    <dc:source>https://www.conicet.gov.ar/</dc:source>
    <skos:narrower rdf:resource="https://vocab.inidep.edu.ar/organizaciones/CENPAT"/>
    <skos:narrower rdf:resource="https://vocab.inidep.edu.ar/organizaciones/CADIC"/>
    <skos:narrower rdf:resource="https://vocab.inidep.edu.ar/organizaciones/IADO"/>
    <skos:narrower rdf:resource="https://vocab.inidep.edu.ar/organizaciones/CIMA"/>
  </rdf:Description>
  <rdf:Description rdf:about="https://vocab.inidep.edu.ar/organizaciones/TAMU">
    <rdf:type rdf:resource="http://www.w3.org/2004/02/skos/core#Concept"/>
    <skos:inScheme rdf:resource="https://vocab.inidep.edu.ar/organizaciones/"/>
    <skos:prefLabel xml:lang="es">Texas A&amp;M University</skos:prefLabel>
    <skos:prefLabel xml:lang="en">Texas A&amp;M University</skos:prefLabel>
    <skos:definition xml:lang="es">Universidad pública de investigación en Texas, EE.UU., con un fuerte programa en oceanografía.</skos:definition>
    <skos:definition xml:lang="en">Public research university in Texas, USA, with a strong program in oceanography.</skos:definition>
    <skos:altLabel xml:lang="en">TAMU</skos:altLabel>
    <dc:source>https://www.tamu.edu/</dc:source>
  </rdf:Description>
  <rdf:Description rdf:about="https://vocab.inidep.edu.ar/organizaciones/">
    <rdf:type rdf:resource="http://www.w3.org/2004/02/skos/core#ConceptScheme"/>
    <dc:title xml:lang="es">tesauro de Organizaciones</dc:title>
    <dc:title xml:lang="en">thesauri of Organizaciones</dc:title>
    <dc:creator>Pablo Rosales</dc:creator>
    <dc:creator>Ana Baldoni</dc:creator>
    <dc:publisher>Universidad Nacional de la Patagonia San Juan Bosco (UNPSJB)</dc:publisher>
    <dc:publisher>Instituto Nacional de Investigación y Desarrollo Pesquero (INIDEP)</dc:publisher>
    <dc:date>2025-07-28</dc:date>
    <skos:hasTopConcept rdf:resource="https://vocab.inidep.edu.ar/organizaciones/INIDEP"/>
    <skos:hasTopConcept rdf:resource="https://vocab.inidep.edu.ar/organizaciones/SHN"/>
    <skos:hasTopConcept rdf:resource="https://vocab.inidep.edu.ar/organizaciones/IFREMER"/>
    <skos:hasTopConcept rdf:resource="https://vocab.inidep.edu.ar/organizaciones/LDGO"/>
    <skos:hasTopConcept rdf:resource="https://vocab.inidep.edu.ar/organizaciones/IAA"/>
    <skos:hasTopConcept rdf:resource="https://vocab.inidep.edu.ar/organizaciones/IEO"/>
    <skos:hasTopConcept rdf:resource="https://vocab.inidep.edu.ar/organizaciones/COPLA"/>
    <skos:hasTopConcept rdf:resource="https://vocab.inidep.edu.ar/organizaciones/CONICET"/>
    <skos:hasTopConcept rdf:resource="https://vocab.inidep.edu.ar/organizaciones/TAMU"/>
    <skos:hasTopConcept rdf:resource="https://vocab.inidep.edu.ar/organizaciones/DINARA"/>
    <skos:hasTopConcept rdf:resource="https://vocab.inidep.edu.ar/organizaciones/FAO"/>
    <skos:hasTopConcept rdf:resource="https://vocab.inidep.edu.ar/organizaciones/COI"/>
    <skos:hasTopConcept rdf:resource="https://vocab.inidep.edu.ar/organizaciones/SAYDS"/>
    <skos:hasTopConcept rdf:resource="https://vocab.inidep.edu.ar/organizaciones/UBA"/>
    <skos:hasTopConcept rdf:resource="https://vocab.inidep.edu.ar/organizaciones/USP"/>
    <skos:hasTopConcept rdf:resource="https://vocab.inidep.edu.ar/organizaciones/UMI-IFAECI"/>
    <skos:hasTopConcept rdf:resource="https://vocab.inidep.edu.ar/organizaciones/ICM"/>
    <skos:hasTopConcept rdf:resource="https://vocab.inidep.edu.ar/organizaciones/OSSE"/>
    <skos:hasTopConcept rdf:resource="https://vocab.inidep.edu.ar/organizaciones/CIMAS"/>
    <skos:hasTopConcept rdf:resource="https://vocab.inidep.edu.ar/organizaciones/SIO"/>
    <skos:hasTopConcept rdf:resource="https://vocab.inidep.edu.ar/organizaciones/AOML"/>
    <skos:hasTopConcept rdf:resource="https://vocab.inidep.edu.ar/organizaciones/FURG"/>
  </rdf:Description>
  <rdf:Description rdf:about="https://vocab.inidep.edu.ar/organizaciones/OSSE">
    <rdf:type rdf:resource="http://www.w3.org/2004/02/skos/core#Concept"/>
    <skos:inScheme rdf:resource="https://vocab.inidep.edu.ar/organizaciones/"/>
    <skos:prefLabel xml:lang="es">Obras Sanitarias Sociedad del Estado MGP</skos:prefLabel>
    <skos:prefLabel xml:lang="en">Obras Sanitarias State Enterprise MGP</skos:prefLabel>
    <skos:definition xml:lang="es">Empresa estatal responsable de los servicios de agua potable y saneamiento en el Partido de General Pueyrredón (Mar del Plata).</skos:definition>
    <skos:definition xml:lang="en">State-owned company responsible for drinking water and sanitation services in the General Pueyrredón district (Mar del Plata).</skos:definition>
    <skos:altLabel xml:lang="en">OSSE</skos:altLabel>
    <dc:source>https://www.osmgp.gov.ar/</dc:source>
  </rdf:Description>
  <rdf:Description rdf:about="https://vocab.inidep.edu.ar/organizaciones/CENPAT">
    <rdf:type rdf:resource="http://www.w3.org/2004/02/skos/core#Concept"/>
    <skos:inScheme rdf:resource="https://vocab.inidep.edu.ar/organizaciones/"/>
    <skos:prefLabel xml:lang="es">Centro Nacional Patagónico -CONICET</skos:prefLabel>
    <skos:prefLabel xml:lang="en">National Patagonian Center -CONICET</skos:prefLabel>
    <skos:definition xml:lang="es">Centro de investigación multidisciplinario del CONICET en Puerto Madryn, enfocado en ecosistemas marinos y terrestres de la Patagonia.</skos:definition>
    <skos:definition xml:lang="en">Multidisciplinary research center of CONICET in Puerto Madryn, focused on marine and terrestrial ecosystems of Patagonia.</skos:definition>
    <skos:altLabel xml:lang="en">CENPAT</skos:altLabel>
    <dc:source>https://cenpat.conicet.gov.ar/</dc:source>
    <skos:broader rdf:resource="https://vocab.inidep.edu.ar/organizaciones/CONICET"/>
  </rdf:Description>
  <rdf:Description rdf:about="https://vocab.inidep.edu.ar/organizaciones/IADO">
    <rdf:type rdf:resource="http://www.w3.org/2004/02/skos/core#Concept"/>
    <skos:inScheme rdf:resource="https://vocab.inidep.edu.ar/organizaciones/"/>
    <skos:prefLabel xml:lang="es">Instituto Argentino de Oceanografía - CONICET</skos:prefLabel>
    <skos:prefLabel xml:lang="en">Argentine Institute of Oceanography - CONICET</skos:prefLabel>
    <skos:definition xml:lang="es">Instituto de investigación del CONICET y la UNS en Bahía Blanca, dedicado a las ciencias marinas.</skos:definition>
    <skos:definition xml:lang="en">Research institute of CONICET and UNS in Bahía Blanca, dedicated to marine sciences.</skos:definition>
    <skos:altLabel xml:lang="en">IADO</skos:altLabel>
    <dc:source>https://iado.conicet.gov.ar/</dc:source>
    <skos:broader rdf:resource="https://vocab.inidep.edu.ar/organizaciones/CONICET"/>
  </rdf:Description>
  <rdf:Description rdf:about="https://vocab.inidep.edu.ar/organizaciones/FAO">
    <rdf:type rdf:resource="http://www.w3.org/2004/02/skos/core#Concept"/>
    <skos:inScheme rdf:resource="https://vocab.inidep.edu.ar/organizaciones/"/>
    <skos:prefLabel xml:lang="es">Organización de las Naciones Unidas para la Alimentación y la Agricultura</skos:prefLabel>
    <skos:prefLabel xml:lang="en">Food and Agriculture Organization of the United Nations</skos:prefLabel>
    <skos:definition xml:lang="es">Agencia especializada de la ONU que lidera los esfuerzos internacionales para vencer el hambre y mejorar la nutrición y la seguridad alimentaria.</skos:definition>
    <skos:definition xml:lang="en">Specialized agency of the UN that leads international efforts to defeat hunger and improve nutrition and food security.</skos:definition>
    <skos:altLabel xml:lang="en">FAO</skos:altLabel>
    <dc:source>https://www.fao.org/</dc:source>
  </rdf:Description>
  <rdf:Description rdf:about="https://vocab.inidep.edu.ar/organizaciones/USP">
    <rdf:type rdf:resource="http://www.w3.org/2004/02/skos/core#Concept"/>
    <skos:inScheme rdf:resource="https://vocab.inidep.edu.ar/organizaciones/"/>
    <skos:prefLabel xml:lang="es">Universidade de São Paulo</skos:prefLabel>
    <skos:prefLabel xml:lang="en">University of São Paulo</skos:prefLabel>
    <skos:definition xml:lang="es">Una de las universidades públicas más importantes de Brasil, con un prestigioso Instituto Oceanográfico.</skos:definition>
    <skos:definition xml:lang="en">One of the most important public universities in Brazil, with a prestigious Oceanographic Institute.</skos:definition>
    <skos:altLabel xml:lang="en">USP</skos:altLabel>
    <dc:source>https://www5.usp.br/</dc:source>
  </rdf:Description>
  <rdf:Description rdf:about="https://vocab.inidep.edu.ar/organizaciones/SAYDS">
    <rdf:type rdf:resource="http://www.w3.org/2004/02/skos/core#Concept"/>
    <skos:inScheme rdf:resource="https://vocab.inidep.edu.ar/organizaciones/"/>
    <skos:prefLabel xml:lang="es">Secretaría de Ambiente y Desarrollo Sustentable</skos:prefLabel>
    <skos:prefLabel xml:lang="en">Secretariat of Environment and Sustainable Development</skos:prefLabel>
    <skos:definition xml:lang="es">Organismo gubernamental a nivel nacional o provincial responsable de las políticas ambientales y de desarrollo sostenible.</skos:definition>
    <skos:definition xml:lang="en">Governmental body at the national or provincial level responsible for environmental and sustainable development policies.</skos:definition>
    <skos:altLabel xml:lang="en">SAyDS</skos:altLabel>
  </rdf:Description>
  <rdf:Description rdf:about="https://vocab.inidep.edu.ar/organizaciones/LDGO">
    <rdf:type rdf:resource="http://www.w3.org/2004/02/skos/core#Concept"/>
    <skos:inScheme rdf:resource="https://vocab.inidep.edu.ar/organizaciones/"/>
    <skos:prefLabel xml:lang="es">Lamont-Doherty Earth Observatory of Columbia University</skos:prefLabel>
    <skos:prefLabel xml:lang="en">Lamont-Doherty Earth Observatory of Columbia University</skos:prefLabel>
    <skos:definition xml:lang="es">Instituto de investigación de la Universidad de Columbia, líder en ciencias de la tierra, clima y océano.</skos:definition>
    <skos:definition xml:lang="en">Research institute of Columbia University, a leader in earth, climate, and ocean sciences.</skos:definition>
    <skos:altLabel xml:lang="en">LDEO</skos:altLabel>
    <dc:source>https://www.ldeo.columbia.edu/</dc:source>
  </rdf:Description>
  <rdf:Description rdf:about="https://vocab.inidep.edu.ar/organizaciones/COI">
    <rdf:type rdf:resource="http://www.w3.org/2004/02/skos/core#Concept"/>
    <skos:inScheme rdf:resource="https://vocab.inidep.edu.ar/organizaciones/"/>
    <skos:prefLabel xml:lang="es">Comisión Oceanográfica Intergubernamental</skos:prefLabel>
    <skos:prefLabel xml:lang="en">Intergovernmental Oceanographic Commission</skos:prefLabel>
    <skos:definition xml:lang="es">Organismo de la UNESCO para las ciencias, los servicios y la observación de los océanos a nivel mundial.</skos:definition>
    <skos:definition xml:lang="en">UNESCO's body for global ocean science, services, and observations.</skos:definition>
    <skos:altLabel xml:lang="en">IOC</skos:altLabel>
    <dc:source>https://ioc.unesco.org/</dc:source>
  </rdf:Description>
  <rdf:Description rdf:about="https://vocab.inidep.edu.ar/organizaciones/CIMA">
    <rdf:type rdf:resource="http://www.w3.org/2004/02/skos/core#Concept"/>
    <skos:inScheme rdf:resource="https://vocab.inidep.edu.ar/organizaciones/"/>
    <skos:prefLabel xml:lang="es">Centro de Investigaciones del Mar y la Atmósfera</skos:prefLabel>
    <skos:prefLabel xml:lang="en">Centre for Atmospheric and Ocean Research</skos:prefLabel>
    <skos:definition xml:lang="es">Instituto de investigación (UBA-CONICET) enfocado en las ciencias de la atmósfera y los océanos.</skos:definition>
    <skos:definition xml:lang="en">Research institute (UBA-CONICET) focused on atmospheric and ocean sciences.</skos:definition>
    <skos:altLabel xml:lang="en">CIMA</skos:altLabel>
    <dc:source>https://www.cima.fcen.uba.ar/</dc:source>
    <skos:broader rdf:resource="https://vocab.inidep.edu.ar/organizaciones/CONICET"/>
  </rdf:Description>
  <rdf:Description rdf:about="https://vocab.inidep.edu.ar/organizaciones/IFREMER">
    <rdf:type rdf:resource="http://www.w3.org/2004/02/skos/core#Concept"/>
    <skos:inScheme rdf:resource="https://vocab.inidep.edu.ar/organizaciones/"/>
    <skos:prefLabel xml:lang="es">Institut Français de Recherche pour l'Exploitation de la Mer</skos:prefLabel>
    <skos:prefLabel xml:lang="en">French Research Institute for Exploitation of the Sea</skos:prefLabel>
    <skos:definition xml:lang="es">Instituto francés de investigación dedicado al conocimiento y la explotación sostenible de los recursos marinos.</skos:definition>
    <skos:definition xml:lang="en">French research institute dedicated to the knowledge and sustainable exploitation of marine resources.</skos:definition>
    <skos:altLabel xml:lang="en">IFREMER</skos:altLabel>
    <dc:source>https://www.ifremer.fr/en/</dc:source>
  </rdf:Description>
  <rdf:Description rdf:about="https://vocab.inidep.edu.ar/organizaciones/INIDEP">
    <rdf:type rdf:resource="http://www.w3.org/2004/02/skos/core#Concept"/>
    <skos:inScheme rdf:resource="https://vocab.inidep.edu.ar/organizaciones/"/>
    <skos:prefLabel xml:lang="es">Instituto Nacional de Investigación y Desarrollo Pesquero</skos:prefLabel>
    <skos:prefLabel xml:lang="en">National Institute for Fisheries Research and Development</skos:prefLabel>
    <skos:definition xml:lang="es">Organismo público de Argentina dedicado a la investigación científica y técnica de los recursos pesqueros y el ambiente marino.</skos:definition>
    <skos:definition xml:lang="en">Public body in Argentina dedicated to the scientific and technical research of fishery resources and the marine environment.</skos:definition>
    <skos:altLabel xml:lang="en">INIDEP</skos:altLabel>
    <dc:source>https://www.argentina.gob.ar/inidep</dc:source>
  </rdf:Description>
  <rdf:Description rdf:about="https://vocab.inidep.edu.ar/organizaciones/CADIC">
    <rdf:type rdf:resource="http://www.w3.org/2004/02/skos/core#Concept"/>
    <skos:inScheme rdf:resource="https://vocab.inidep.edu.ar/organizaciones/"/>
    <skos:prefLabel xml:lang="es">Centro Austral de Investigaciones Científicas -CONICET</skos:prefLabel>
    <skos:prefLabel xml:lang="en">Austral Center for Scientific Research -CONICET</skos:prefLabel>
    <skos:definition xml:lang="es">Centro de investigación multidisciplinario del CONICET en Ushuaia, dedicado al estudio de los sistemas subantárticos.</skos:definition>
    <skos:definition xml:lang="en">Multidisciplinary research center of CONICET in Ushuaia, dedicated to the study of subantarctic systems.</skos:definition>
    <skos:altLabel xml:lang="en">CADIC</skos:altLabel>
    <dc:source>https://cadic.conicet.gov.ar/</dc:source>
    <skos:broader rdf:resource="https://vocab.inidep.edu.ar/organizaciones/CONICET"/>
  </rdf:Description>
  <rdf:Description rdf:about="https://vocab.inidep.edu.ar/organizaciones/FURG">
    <rdf:type rdf:resource="http://www.w3.org/2004/02/skos/core#Concept"/>
    <skos:inScheme rdf:resource="https://vocab.inidep.edu.ar/organizaciones/"/>
    <skos:prefLabel xml:lang="es">Universidade Federal do Rio Grande</skos:prefLabel>
    <skos:prefLabel xml:lang="en">Federal University of Rio Grande</skos:prefLabel>
    <skos:definition xml:lang="es">Universidad pública brasileña en Rio Grande, con un fuerte enfoque en las ciencias marinas y la oceanografía.</skos:definition>
    <skos:definition xml:lang="en">A Brazilian public university in Rio Grande, with a strong focus on marine sciences and oceanography.</skos:definition>
    <skos:altLabel xml:lang="en">FURG</skos:altLabel>
    <dc:source>https://www.furg.br/</dc:source>
  </rdf:Description>
  <rdf:Description rdf:about="https://vocab.inidep.edu.ar/organizaciones/SHN">
    <rdf:type rdf:resource="http://www.w3.org/2004/02/skos/core#Concept"/>
    <skos:inScheme rdf:resource="https://vocab.inidep.edu.ar/organizaciones/"/>
    <skos:prefLabel xml:lang="es">Servicio de Hidrografía Naval</skos:prefLabel>
    <skos:prefLabel xml:lang="en">Naval Hydrographic Service</skos:prefLabel>
    <skos:definition xml:lang="es">Organismo de la Armada Argentina responsable de la seguridad náutica, la cartografía marina y la investigación oceanográfica.</skos:definition>
    <skos:definition xml:lang="en">Agency of the Argentine Navy responsible for nautical safety, marine cartography, and oceanographic research.</skos:definition>
    <skos:altLabel xml:lang="en">SHN</skos:altLabel>
    <dc:source>https://www.hidro.gob.ar/</dc:source>
  </rdf:Description>
  <rdf:Description rdf:about="https://vocab.inidep.edu.ar/organizaciones/AOML">
    <rdf:type rdf:resource="http://www.w3.org/2004/02/skos/core#Concept"/>
    <skos:inScheme rdf:resource="https://vocab.inidep.edu.ar/organizaciones/"/>
    <skos:prefLabel xml:lang="es">Atlantic Oceanographic and Meteorological Laboratory</skos:prefLabel>
    <skos:prefLabel xml:lang="en">Atlantic Oceanographic and Meteorological Laboratory</skos:prefLabel>
    <skos:definition xml:lang="es">Laboratorio de investigación de la NOAA en Miami, EE.UU., que estudia los océanos y la atmósfera del Atlántico.</skos:definition>
    <skos:definition xml:lang="en">A research laboratory of NOAA in Miami, USA, that studies the Atlantic oceans and atmosphere.</skos:definition>
    <skos:altLabel xml:lang="en">AOML</skos:altLabel>
    <dc:source>https://www.aoml.noaa.gov/</dc:source>
  </rdf:Description>
  <rdf:Description rdf:about="https://vocab.inidep.edu.ar/organizaciones/DINARA">
    <rdf:type rdf:resource="http://www.w3.org/2004/02/skos/core#Concept"/>
    <skos:inScheme rdf:resource="https://vocab.inidep.edu.ar/organizaciones/"/>
    <skos:prefLabel xml:lang="es">Dirección Nacional de Recursos Acuáticos</skos:prefLabel>
    <skos:prefLabel xml:lang="en">National Directorate of Aquatic Resources</skos:prefLabel>
    <skos:definition xml:lang="es">Organismo de Uruguay responsable de la regulación y fomento del sector pesquero y acuícola.</skos:definition>
    <skos:definition xml:lang="en">Uruguayan agency responsible for the regulation and promotion of the fishing and aquaculture sector.</skos:definition>
    <skos:altLabel xml:lang="en">DINARA</skos:altLabel>
    <dc:source>https://www.gub.uy/direccion-nacional-recursos-acuaticos/</dc:source>
  </rdf:Description>
  <rdf:Description rdf:about="https://vocab.inidep.edu.ar/organizaciones/UMI-IFAECI">
    <rdf:type rdf:resource="http://www.w3.org/2004/02/skos/core#Concept"/>
    <skos:inScheme rdf:resource="https://vocab.inidep.edu.ar/organizaciones/"/>
    <skos:prefLabel xml:lang="es">Instituto Franco-Argentino sobre Estudios de Clima y sus Impactos</skos:prefLabel>
    <skos:prefLabel xml:lang="en">French-Argentine Institute on Climate Studies and their Impacts</skos:prefLabel>
    <skos:definition xml:lang="es">Centro de investigación binacional (Argentina-Francia) dedicado al estudio de la variabilidad y el cambio climático.</skos:definition>
    <skos:definition xml:lang="en">Bi-national research center (Argentina-France) dedicated to the study of climate variability and change.</skos:definition>
    <skos:altLabel xml:lang="en">UMI-IFAECI</skos:altLabel>
    <dc:source>http://www.ifaeci.cnrs.fr/</dc:source>
  </rdf:Description>
  <rdf:Description rdf:about="https://vocab.inidep.edu.ar/organizaciones/IEO">
    <rdf:type rdf:resource="http://www.w3.org/2004/02/skos/core#Concept"/>
    <skos:inScheme rdf:resource="https://vocab.inidep.edu.ar/organizaciones/"/>
    <skos:prefLabel xml:lang="es">Instituto Español de Oceanografía</skos:prefLabel>
    <skos:prefLabel xml:lang="en">Spanish Institute of Oceanography</skos:prefLabel>
    <skos:definition xml:lang="es">Organismo público de investigación de España dedicado al estudio de los mares y sus recursos.</skos:definition>
    <skos:definition xml:lang="en">Public research organization in Spain dedicated to the study of the seas and their resources.</skos:definition>
    <skos:altLabel xml:lang="en">IEO</skos:altLabel>
    <dc:source>https://www.ieo.csic.es/</dc:source>
  </rdf:Description>
  <rdf:Description rdf:about="https://vocab.inidep.edu.ar/organizaciones/ICM">
    <rdf:type rdf:resource="http://www.w3.org/2004/02/skos/core#Concept"/>
    <skos:inScheme rdf:resource="https://vocab.inidep.edu.ar/organizaciones/"/>
    <skos:prefLabel xml:lang="es">Institut de Ciències del Mar de Barcelona</skos:prefLabel>
    <skos:prefLabel xml:lang="en">Institute of Marine Sciences of Barcelona</skos:prefLabel>
    <skos:definition xml:lang="es">Centro de investigación marina del CSIC ubicado en Barcelona, España.</skos:definition>
    <skos:definition xml:lang="en">Marine research center of the CSIC located in Barcelona, Spain.</skos:definition>
    <skos:altLabel xml:lang="en">ICM</skos:altLabel>
    <dc:source>https://www.icm.csic.es/</dc:source>
  </rdf:Description>
  <rdf:Description rdf:about="https://vocab.inidep.edu.ar/organizaciones/COPLA">
    <rdf:type rdf:resource="http://www.w3.org/2004/02/skos/core#Concept"/>
    <skos:inScheme rdf:resource="https://vocab.inidep.edu.ar/organizaciones/"/>
    <skos:prefLabel xml:lang="es">Comisión Nacional del Límite Exterior de la Plataforma Continental</skos:prefLabel>
    <skos:prefLabel xml:lang="en">National Commission on the Outer Limit of the Continental Shelf</skos:prefLabel>
    <skos:definition xml:lang="es">Comisión del gobierno argentino encargada de establecer el límite exterior de la plataforma continental argentina.</skos:definition>
    <skos:definition xml:lang="en">Argentine government commission responsible for establishing the outer limit of the Argentine continental shelf.</skos:definition>
    <skos:altLabel xml:lang="en">COPLA</skos:altLabel>
    <dc:source>https://www.argentina.gob.ar/copla</dc:source>
  </rdf:Description>
  <rdf:Description rdf:about="https://vocab.inidep.edu.ar/organizaciones/SIO">
    <rdf:type rdf:resource="http://www.w3.org/2004/02/skos/core#Concept"/>
    <skos:inScheme rdf:resource="https://vocab.inidep.edu.ar/organizaciones/"/>
    <skos:prefLabel xml:lang="es">Scripps Institution of Oceanography</skos:prefLabel>
    <skos:prefLabel xml:lang="en">Scripps Institution of Oceanography</skos:prefLabel>
    <skos:definition xml:lang="es">Una de las instituciones de investigación oceanográfica más antiguas y grandes del mundo, parte de la Universidad de California, San Diego.</skos:definition>
    <skos:definition xml:lang="en">One of the world's oldest and largest oceanographic research institutions, part of the University of California, San Diego.</skos:definition>
    <skos:altLabel xml:lang="en">SIO</skos:altLabel>
    <dc:source>https://scripps.ucsd.edu/</dc:source>
  </rdf:Description>
</rdf:RDF>
